

Q 1

$$Mgf_{X+Y} = Mgf_X \times Mgf_Y$$

$$\text{now } M_{X+Y}(t) = E(e^{t(X+Y)}) = E(e^{tx} \times e^{ty})$$

Now X and Y are independent so

e^{tx} and e^{ty} are also independent then

$$M_{X+Y}(t) = E(e^{tx} e^{ty}) = E(e^{tx}) E(e^{ty}) = M_X(t) M_Y(t)$$

Finding the distrib of $Y = \sum X_i/n$ for $X_i \sim N(\mu, \sigma^2)$

Ans:

$Y = \sum X_i/n$ X_i : is a random independent variable observing pdf: N

$$X_i \sim N(\mu, \sigma^2)$$

$$X'_i = \frac{X_i}{n} \sim N\left(\frac{\mu}{n}, \frac{\sigma^2}{n^2}\right)$$

$$\begin{aligned} M_{X'_i}(t) &= \int_{-\infty}^{\infty} e^{tx} \frac{1}{\sqrt{2\pi}} \frac{n}{\sigma} e^{-\frac{(x - \mu/n)^2}{2(\sigma/n)^2}} dx \\ &= e^{\mu/n t + \frac{\sigma^2 t^2}{2n^2}} \end{aligned}$$

Now WKT for $Z = X + Y$, X, Y independent

$$M_Z(t) = M_X(t) \cdot M_Y(t).$$

\therefore We can say that,

$$\begin{aligned} M_Y &= M_{X'_1} M_{X'_2} M_{X'_3} M_{X'_4} \cdots M_{X'_n} \\ &= \prod_{i=1}^n M_{X'_i}(t). \end{aligned}$$

$$M_Y = \left(e^{\mu/n t + \frac{\sigma^2 t^2}{2n^2}} \right)^n = e^{\mu t + \frac{\sigma^2}{n} t^2/2}$$

By observation we can see that M_Y is comparable to the MGF of pdf: $N(\mu, \sigma^2/n)$.

$$\therefore \text{pdf: } Y \sim N\left(\mu, \frac{\sigma^2}{n}\right).$$

Q3 $X_1 \sim \text{Exp}(1)$

$$f_{X_1}(x) = e^{-x} \quad x > 0$$

Q. $M_X(t) = E(e^{tx}) = \int_0^{\infty} e^{tx} e^{-x} dx$

$$M_X(t) = \int_0^{\infty} e^{-(1-t)x} dx$$

this integration is only well defined when $t < 1$

$$M_X(t) = \frac{1}{1-t}$$

$$Y = \sum X_i$$

$$M_Y(t) = \prod M_{X_i}(t) = \left(\frac{1}{1-t} \right)^n$$

Now $Z \sim \text{Gamma}(n, 1)$

$$f_Z(x) = \frac{1}{\Gamma(n)} x^{n-1} e^{-x} \quad x > 0$$

$$M_Z(t) = \int_0^{\infty} \frac{1}{\Gamma(n)} x^{n-1} e^{-(1-t)x} dx$$

Now we know $\int_0^{\infty} x^{a-1} e^{-bx} dx = \frac{\Gamma(a)}{(b)^a}$

$$\text{so } M_Z(t) = \frac{1}{(1-t)^n} = M_Y(t)$$

so $Z \sim Y$